SeqHigherLevel.dfy
@@ -1,6 +1,6 @@
 module SeqHigherLevel { 
   // applies a transformation function on the sequence
-  function method {:opaque} Map<E,R>(f: (E ~> R), s: seq<E>): (result: seq<R>)
+  function method {:opaque} Map<T,R>(f: (T ~> R), s: seq<T>): (result: seq<R>)
     requires forall i :: 0 <= i < |s| ==> f.requires(s[i])
     ensures |result| == |s|
     ensures forall i :: 0 <= i < |s| ==> result[i] == f(s[i]);
@@ -11,7 +11,7 @@ module SeqHigherLevel {
   }
 
   // uses a selection function to select elements from the sequence
-  function method {:opaque} filter<E>(f : (E ~> bool), s: seq<E>): (result: seq<E>)
+  function method {:opaque} filter<T>(f : (T ~> bool), s: seq<T>): (result: seq<T>)
     requires forall i :: 0 <= i < |s| ==> f.requires(s[i])
     ensures |result| <= |s|
     ensures forall i: nat :: i < |result| && f.requires(result[i]) ==> f(result[i])
@@ -21,13 +21,13 @@ module SeqHigherLevel {
     else ((if f(s[0]) then [s[0]] else []) + filter(f, s[1..]))
   }
   
-  function method {:opaque} fold_left<A,E>(f: (A, E) -> A, init: A, s: seq<E>): A
+  function method {:opaque} fold_left<A,T>(f: (A, T) -> A, init: A, s: seq<T>): A
   {
     if |s| == 0 then init
     else fold_left(f, f(init, s[0]), s[1..])
   }
 
-  function method {:opaque} fold_right<A,E>(f: (A, E) -> A, init: A, s: seq<E>): A
+  function method {:opaque} fold_right<A,T>(f: (A, T) -> A, init: A, s: seq<T>): A
   {
     if |s| == 0 then init
     else f(fold_right(f, init, s[1..]), s[0])
