SeqLast.dfy
@@ -1,14 +1,14 @@
 module SeqLast {
 
   // returns the last element in the sequence
-  function method last<E>(s: seq<E>): E
+  function method last<T>(s: seq<T>): T
     requires |s| > 0;
   {
     s[|s|-1]
   }
 
   // returns the sequence slice up to but not including the last element
-  function method drop_last<E>(s: seq<E>): seq<E> 
+  function method drop_last<T>(s: seq<T>): seq<T> 
   requires |s| > 0;
   {
     s[..|s|-1]
